theories/zoo_std/xtchain.v
@@ -19,222 +19,343 @@ Implicit Types v next dst : val.
 Section zoo_G.
   Context `{zoo_G : !ZooG Σ}.
 
-  Definition xtchain hdr nodes dst : iProp Σ :=
-    xchain nodes dst ∗
+  Definition xtchain hdr dq nodes dst : iProp Σ :=
+    xchain dq nodes dst ∗
     [∗ list] node ∈ nodes, node ↦ₕ hdr.
 
-  #[global] Instance xtchain_timeless hdr nodes dst :
-    Timeless (xtchain hdr nodes dst).
+  #[global] Instance xtchain_timeless hdr dq nodes dst :
+    Timeless (xtchain hdr dq nodes dst).
+  Proof.
+    apply _.
+  Qed.
+  #[global] Instance xtchain_persistent hdr nodes dst :
+    Persistent (xtchain hdr DfracDiscarded nodes dst).
   Proof.
     apply _.
   Qed.
 
-  Lemma xtchain_nil hdr dst :
-    ⊢ xtchain hdr [] dst.
+  Lemma xtchain_nil hdr dq dst :
+    ⊢ xtchain hdr dq [] dst.
   Proof.
     iSteps.
   Qed.
 
-  Lemma xtchain_singleton hdr node dst :
-    xtchain hdr [node] dst ⊣⊢
+  Lemma xtchain_singleton hdr dq node dst :
+    xtchain hdr dq [node] dst ⊣⊢
       node ↦ₕ hdr ∗
-      node.[xtchain_next] ↦ dst.
+      node.[xtchain_next] ↦{dq} dst.
   Proof.
     rewrite /xtchain xchain_singleton. iSteps.
   Qed.
-  Lemma xtchain_singleton_1 hdr node dst :
-    xtchain hdr [node] dst ⊢
+  Lemma xtchain_singleton_1 hdr dq node dst :
+    xtchain hdr dq [node] dst ⊢
       node ↦ₕ hdr ∗
-      node.[xtchain_next] ↦ dst.
+      node.[xtchain_next] ↦{dq} dst.
   Proof.
     rewrite xtchain_singleton //.
   Qed.
-  Lemma xtchain_singleton_2 hdr node dst :
+  Lemma xtchain_singleton_2 hdr dq node dst :
     node ↦ₕ hdr ∗
-    node.[xtchain_next] ↦ dst -∗
-    xtchain hdr [node] dst.
+    node.[xtchain_next] ↦{dq} dst -∗
+    xtchain hdr dq [node] dst.
   Proof.
     rewrite -xtchain_singleton. auto.
   Qed.
 
-  Lemma xtchain_cons {hdr} nodes node nodes' dst :
+  Lemma xtchain_cons {hdr dq} nodes node nodes' dst :
     nodes = node :: nodes' →
-    xtchain hdr nodes dst ⊣⊢
+    xtchain hdr dq nodes dst ⊣⊢
       node ↦ₕ hdr ∗
-      node.[xtchain_next] ↦ from_option #@{location} dst (head nodes') ∗
-      xtchain hdr nodes' dst.
+      node.[xtchain_next] ↦{dq} from_option #@{location} dst (head nodes') ∗
+      xtchain hdr dq nodes' dst.
   Proof.
     intros ->.
     rewrite /xtchain xchain_cons // big_sepL_cons. iSteps.
   Qed.
-  Lemma xtchain_cons_1 {hdr} nodes node nodes' dst :
-    nodes = node :: nodes' →
-    xtchain hdr nodes dst ⊢
+  Lemma xtchain_cons' {hdr dq} node nodes dst :
+    xtchain hdr dq (node :: nodes) dst ⊣⊢
       node ↦ₕ hdr ∗
-      node.[xtchain_next] ↦ from_option #@{location} dst (head nodes') ∗
-      xtchain hdr nodes' dst.
+      node.[xtchain_next] ↦{dq} from_option #@{location} dst (head nodes) ∗
+      xtchain hdr dq nodes dst.
   Proof.
-    intros. rewrite xtchain_cons //.
+    rewrite xtchain_cons //.
   Qed.
-  Lemma xtchain_cons_2 hdr node nodes dst :
-    node ↦ₕ hdr ∗
-    node.[xtchain_next] ↦ from_option #@{location} dst (head nodes) -∗
-    xtchain hdr nodes dst -∗
-    xtchain hdr (node :: nodes) dst.
+  Lemma xtchain_cons_1 {hdr dq} nodes node nodes' dst :
+    nodes = node :: nodes' →
+    xtchain hdr dq nodes dst ⊢
+      node ↦ₕ hdr ∗
+      node.[xtchain_next] ↦{dq} from_option #@{location} dst (head nodes') ∗
+      xtchain hdr dq nodes' dst.
+  Proof.
+    intros.
+    rewrite xtchain_cons //.
+  Qed.
+  Lemma xtchain_cons_1' {hdr dq} node nodes dst :
+    xtchain hdr dq (node :: nodes) dst ⊢
+      node ↦ₕ hdr ∗
+      node.[xtchain_next] ↦{dq} from_option #@{location} dst (head nodes) ∗
+      xtchain hdr dq nodes dst.
+  Proof.
+    rewrite xtchain_cons //.
+  Qed.
+  Lemma xtchain_cons_2 hdr dq node nodes dst :
+    node ↦ₕ hdr -∗
+    node.[xtchain_next] ↦{dq} from_option #@{location} dst (head nodes) -∗
+    xtchain hdr dq nodes dst -∗
+    xtchain hdr dq (node :: nodes) dst.
   Proof.
     rewrite (xtchain_cons (node :: nodes)) //. iSteps.
   Qed.
 
-  Lemma xtchain_app {hdr} nodes nodes1 nodes2 dst :
+  Lemma xtchain_app {hdr dq} nodes nodes1 nodes2 dst :
     nodes = nodes1 ++ nodes2 →
-    xtchain hdr nodes dst ⊣⊢
-      xtchain hdr nodes1 (from_option #@{location} dst (head nodes2)) ∗
-      xtchain hdr nodes2 dst.
+    xtchain hdr dq nodes dst ⊣⊢
+      xtchain hdr dq nodes1 (from_option #@{location} dst (head nodes2)) ∗
+      xtchain hdr dq nodes2 dst.
   Proof.
     intros ->.
     rewrite /xtchain xchain_app // big_sepL_app. iSteps.
   Qed.
-  Lemma xtchain_app_1 {hdr} nodes nodes1 nodes2 dst :
-    nodes = nodes1 ++ nodes2 →
-    xtchain hdr nodes dst ⊢
-      xtchain hdr nodes1 (from_option #@{location} dst (head nodes2)) ∗
-      xtchain hdr nodes2 dst.
+  Lemma xtchain_app' {hdr dq} nodes1 nodes2 dst :
+    xtchain hdr dq (nodes1 ++ nodes2) dst ⊣⊢
+      xtchain hdr dq nodes1 (from_option #@{location} dst (head nodes2)) ∗
+      xtchain hdr dq nodes2 dst.
   Proof.
-    intros. rewrite xtchain_app //.
+    rewrite xtchain_app //.
   Qed.
-  Lemma xtchain_app_2 hdr nodes1 nodes2 dst :
-    xtchain hdr nodes1 (from_option #@{location} dst (head nodes2)) -∗
-    xtchain hdr nodes2 dst -∗
-    xtchain hdr (nodes1 ++ nodes2) dst.
+  Lemma xtchain_app_1 {hdr dq} nodes nodes1 nodes2 dst :
+    nodes = nodes1 ++ nodes2 →
+    xtchain hdr dq nodes dst ⊢
+      xtchain hdr dq nodes1 (from_option #@{location} dst (head nodes2)) ∗
+      xtchain hdr dq nodes2 dst.
+  Proof.
+    intros.
+    rewrite xtchain_app //.
+  Qed.
+  Lemma xtchain_app_1' {hdr dq} nodes1 nodes2 dst :
+    xtchain hdr dq (nodes1 ++ nodes2) dst ⊢
+      xtchain hdr dq nodes1 (from_option #@{location} dst (head nodes2)) ∗
+      xtchain hdr dq nodes2 dst.
+  Proof.
+    rewrite xtchain_app //.
+  Qed.
+  Lemma xtchain_app_2 hdr dq nodes1 nodes2 dst :
+    xtchain hdr dq nodes1 (from_option #@{location} dst (head nodes2)) -∗
+    xtchain hdr dq nodes2 dst -∗
+    xtchain hdr dq (nodes1 ++ nodes2) dst.
   Proof.
     rewrite (xtchain_app (nodes1 ++ nodes2)) //. iSteps.
   Qed.
 
-  Lemma xtchain_snoc {hdr} nodes nodes' node dst :
+  Lemma xtchain_snoc {hdr dq} nodes nodes' node dst :
     nodes = nodes' ++ [node] →
-    xtchain hdr nodes dst ⊣⊢
-      xtchain hdr nodes' #node ∗
+    xtchain hdr dq nodes dst ⊣⊢
+      xtchain hdr dq nodes' #node ∗
       node ↦ₕ hdr ∗
-      node.[xtchain_next] ↦ dst.
+      node.[xtchain_next] ↦{dq} dst.
   Proof.
     intros ->.
     rewrite /xtchain xchain_snoc // big_sepL_snoc. iSteps.
   Qed.
-  Lemma xtchain_snoc_1 {hdr} nodes nodes' node dst :
-    nodes = nodes' ++ [node] →
-    xtchain hdr nodes dst ⊢
-      xtchain hdr nodes' #node ∗
+  Lemma xtchain_snoc' {hdr dq} nodes node dst :
+    xtchain hdr dq (nodes ++ [node]) dst ⊣⊢
+      xtchain hdr dq nodes #node ∗
       node ↦ₕ hdr ∗
-      node.[xtchain_next] ↦ dst.
+      node.[xtchain_next] ↦{dq} dst.
   Proof.
-    intros. rewrite xtchain_snoc //.
+    rewrite xtchain_snoc //.
   Qed.
-  Lemma xtchain_snoc_2 hdr nodes node dst :
-    xtchain hdr nodes #node -∗
+  Lemma xtchain_snoc_1 {hdr dq} nodes nodes' node dst :
+    nodes = nodes' ++ [node] →
+    xtchain hdr dq nodes dst ⊢
+      xtchain hdr dq nodes' #node ∗
+      node ↦ₕ hdr ∗
+      node.[xtchain_next] ↦{dq} dst.
+  Proof.
+    intros.
+    rewrite xtchain_snoc //.
+  Qed.
+  Lemma xtchain_snoc_1' {hdr dq} nodes node dst :
+    xtchain hdr dq (nodes ++ [node]) dst ⊢
+      xtchain hdr dq nodes #node ∗
+      node ↦ₕ hdr ∗
+      node.[xtchain_next] ↦{dq} dst.
+  Proof.
+    rewrite xtchain_snoc //.
+  Qed.
+  Lemma xtchain_snoc_2 hdr dq nodes node dst :
+    xtchain hdr dq nodes #node -∗
     node ↦ₕ hdr -∗
-    node.[xtchain_next] ↦ dst -∗
-    xtchain hdr (nodes ++ [node]) dst.
+    node.[xtchain_next] ↦{dq} dst -∗
+    xtchain hdr dq (nodes ++ [node]) dst.
   Proof.
     rewrite (xtchain_snoc (nodes ++ [node])) //. iSteps.
   Qed.
 
-  Lemma xtchain_lookup {hdr nodes} i node dst :
+  Lemma xtchain_lookup {hdr dq nodes} i node dst :
     nodes !! i = Some node →
-    xtchain hdr nodes dst ⊣⊢
-      xtchain hdr (take i nodes) #node ∗
+    xtchain hdr dq nodes dst ⊣⊢
+      xtchain hdr dq (take i nodes) #node ∗
       node ↦ₕ hdr ∗
-      node.[xtchain_next] ↦ from_option #@{location} dst (nodes !! S i) ∗
-      xtchain hdr (drop (S i) nodes) dst.
+      node.[xtchain_next] ↦{dq} from_option #@{location} dst (nodes !! S i) ∗
+      xtchain hdr dq (drop (S i) nodes) dst.
   Proof.
     intros.
     rewrite /xtchain xchain_lookup //.
     rewrite -{4}(take_drop_middle nodes i node) // big_sepL_app.
     iSteps.
   Qed.
-  Lemma xtchain_lookup_1 {hdr nodes} i node dst :
+  Lemma xtchain_lookup_1 {hdr dq nodes} i node dst :
     nodes !! i = Some node →
-    xtchain hdr nodes dst ⊢
-      xtchain hdr (take i nodes) #node ∗
+    xtchain hdr dq nodes dst ⊢
+      xtchain hdr dq (take i nodes) #node ∗
       node ↦ₕ hdr ∗
-      node.[xtchain_next] ↦ from_option #@{location} dst (nodes !! S i) ∗
-      xtchain hdr (drop (S i) nodes) dst.
+      node.[xtchain_next] ↦{dq} from_option #@{location} dst (nodes !! S i) ∗
+      xtchain hdr dq (drop (S i) nodes) dst.
   Proof.
-    intros. rewrite xtchain_lookup //.
+    intros.
+    rewrite xtchain_lookup //.
   Qed.
-  Lemma xtchain_lookup_2 {hdr nodes} i node next dst :
+  Lemma xtchain_lookup_2 {hdr dq nodes} i node next dst :
     nodes !! i = Some node →
     next = from_option #@{location} dst (nodes !! S i) →
-    xtchain hdr (take i nodes) #node -∗
+    xtchain hdr dq (take i nodes) #node -∗
     node ↦ₕ hdr -∗
-    node.[xtchain_next] ↦ next -∗
-    xtchain hdr (drop (S i) nodes) dst -∗
-    xtchain hdr nodes dst.
+    node.[xtchain_next] ↦{dq} next -∗
+    xtchain hdr dq (drop (S i) nodes) dst -∗
+    xtchain hdr dq nodes dst.
   Proof.
-    intros. rewrite (@xtchain_lookup _ nodes) //. iSteps.
+    intros. subst.
+    rewrite (@xtchain_lookup _ _ nodes) //. iSteps.
   Qed.
 
-  Lemma xtchain_lookup_acc {hdr nodes} i node dst :
+  Lemma xtchain_lookup_acc {hdr dq nodes} i node dst :
     nodes !! i = Some node →
-    xtchain hdr nodes dst ⊢
+    xtchain hdr dq nodes dst ⊢
       node ↦ₕ hdr ∗
-      node.[xtchain_next] ↦ from_option #@{location} dst (nodes !! S i) ∗
-      ( node.[xtchain_next] ↦ from_option #@{location} dst (nodes !! S i) -∗
-        xtchain hdr nodes dst
+      node.[xtchain_next] ↦{dq} from_option #@{location} dst (nodes !! S i) ∗
+      ( node.[xtchain_next] ↦{dq} from_option #@{location} dst (nodes !! S i) -∗
+        xtchain hdr dq nodes dst
       ).
   Proof.
     intros. rewrite xtchain_lookup //. iSteps.
   Qed.
 
-  Lemma xtchain_lookup_header {hdr nodes} i node dst :
+  Lemma xtchain_lookup_header {hdr dq nodes} i node dst :
     nodes !! i = Some node →
-    xtchain hdr nodes dst ⊢
+    xtchain hdr dq nodes dst ⊢
     node ↦ₕ hdr.
   Proof.
     intros. rewrite xtchain_lookup //. iSteps.
   Qed.
 
-  Lemma xtchain_exclusive hdr nodes dst1 dst2 :
+  Lemma xtchain_valid hdr dq nodes dst :
     0 < length nodes →
-    xtchain hdr nodes dst1 -∗
-    xtchain hdr nodes dst2 -∗
+    xtchain hdr dq nodes dst ⊢
+    ⌜✓ dq⌝.
+  Proof.
+    iIntros "% (H & _)".
+    iApply (xchain_valid with "H"); first done.
+  Qed.
+  Lemma xtchain_combine hdr nodes dq1 dst1 dq2 dst2 :
+    0 < length nodes →
+    xtchain hdr dq1 nodes dst1 -∗
+    xtchain hdr dq2 nodes dst2 -∗
+      ⌜dst1 = dst2⌝ ∗
+      xtchain hdr (dq1 ⋅ dq2) nodes dst1.
+  Proof.
+    iIntros "% (H1 & $) (H2 & _)".
+    iApply (xchain_combine with "H1 H2"); first done.
+  Qed.
+  Lemma xtchain_valid_2 hdr nodes dq1 dst1 dq2 dst2 :
+    0 < length nodes →
+    xtchain hdr dq1 nodes dst1 -∗
+    xtchain hdr dq2 nodes dst2 -∗
+      ⌜✓ (dq1 ⋅ dq2)⌝ ∗
+      ⌜dst1 = dst2⌝.
+  Proof.
+    iIntros "% H1 H2".
+    iDestruct (xtchain_combine with "H1 H2") as "(-> & H)"; first done.
+    iDestruct (xtchain_valid with "H") as "$"; first done.
+    iSteps.
+  Qed.
+  Lemma xtchain_agree hdr nodes dq1 dst1 dq2 dst2 :
+    0 < length nodes →
+    xtchain hdr dq1 nodes dst1 -∗
+    xtchain hdr dq2 nodes dst2 -∗
+    ⌜dst1 = dst2⌝.
+  Proof.
+    iIntros "% H1 H2".
+    iDestruct (xtchain_combine with "H1 H2") as "($ & _)"; first done.
+  Qed.
+  Lemma xtchain_dfrac_ne hdr dq1 nodes1 dst1 dq2 nodes2 dst2 :
+    0 < length nodes1 →
+    ¬ ✓ (dq1 ⋅ dq2) →
+    xtchain hdr dq1 nodes1 dst1 -∗
+    xtchain hdr dq2 nodes2 dst2 -∗
+    ⌜nodes1 ≠ nodes2⌝.
+  Proof.
+    iIntros "% % H1 H2" (->).
+    iDestruct (xtchain_valid_2 with "H1 H2") as %?; naive_solver.
+  Qed.
+  Lemma xtchain_ne hdr nodes1 dst1 dq2 nodes2 dst2 :
+    0 < length nodes1 →
+    xtchain hdr (DfracOwn 1) nodes1 dst1 -∗
+    xtchain hdr dq2 nodes2 dst2 -∗
+    ⌜nodes1 ≠ nodes2⌝.
+  Proof.
+    intros.
+    iApply xtchain_dfrac_ne; [done.. | intros []%(exclusive_l _)].
+  Qed.
+  Lemma xtchain_exclusive hdr nodes dst1 dq2 dst2 :
+    0 < length nodes →
+    xtchain hdr (DfracOwn 1) nodes dst1 -∗
+    xtchain hdr dq2 nodes dst2 -∗
     False.
   Proof.
-    iIntros "% (H1 & _) (H2 & _)".
-    iApply (xchain_exclusive with "H1 H2"); first done.
+    iIntros "% H1 H2".
+    iDestruct (xtchain_ne with "H1 H2") as %?; done.
+  Qed.
+  Lemma xtchain_persist hdr dq nodes dst :
+    xtchain hdr dq nodes dst ⊢ |==>
+    xtchain hdr DfracDiscarded nodes dst.
+  Proof.
+    iIntros "(H & $)".
+    iApply (xchain_persist with "H").
   Qed.
 
   Lemma xtchain_NoDup hdr nodes dst :
-    xtchain hdr nodes dst ⊢
+    xtchain hdr (DfracOwn 1) nodes dst ⊢
     ⌜NoDup nodes⌝.
   Proof.
     iIntros "(H & _)".
     iApply (xchain_NoDup with "H").
   Qed.
 
-  Lemma xtchain_next_spec {hdr nodes node} nodes' dst E :
+  Lemma xtchain_next_spec {hdr dq nodes node} nodes' dst E :
     nodes = node :: nodes' →
     {{{
-      xtchain hdr nodes dst
+      xtchain dq hdr nodes dst
     }}}
       (#node).{xtchain_next} @ E
     {{{
       RET from_option #@{location} dst (head nodes');
-      xtchain hdr nodes dst
+      xtchain dq hdr nodes dst
     }}}.
   Proof.
     iIntros (->) "%Φ (H & Hheaders) HΦ".
     wp_apply (xchain_next_spec with "H"); first done.
     iSteps.
   Qed.
-  Lemma xtchain_next_spec_lookup {hdr nodes} i node dst E :
+  Lemma xtchain_next_spec_lookup {hdr dq nodes} i node dst E :
     nodes !! i = Some node →
     {{{
-      xtchain hdr nodes dst
+      xtchain hdr dq nodes dst
     }}}
       (#node).{xtchain_next} @ E
     {{{
       RET from_option #@{location} dst (nodes !! S i);
-      xtchain hdr nodes dst
+      xtchain hdr dq nodes dst
     }}}.
   Proof.
     iIntros "%Hlookup %Φ (H & Hheaders) HΦ".
@@ -245,13 +366,13 @@ Section zoo_G.
   Lemma xtchain_set_next_spec {hdr nodes node} nodes' dst v E :
     nodes = node :: nodes' →
     {{{
-      xtchain hdr nodes dst
+      xtchain hdr (DfracOwn 1) nodes dst
     }}}
       (#node) <-{xtchain_next} v @ E
     {{{
       RET ();
-      xtchain hdr [node] v ∗
-      xtchain hdr nodes' dst
+      xtchain hdr (DfracOwn 1) [node] v ∗
+      xtchain hdr (DfracOwn 1) nodes' dst
     }}}.
   Proof.
     iIntros (->) "%Φ (H & Hheaders) HΦ".
@@ -261,13 +382,13 @@ Section zoo_G.
   Lemma xtchain_set_next_spec_lookup {hdr nodes} i node dst v E :
     nodes !! i = Some node →
     {{{
-      xtchain hdr nodes dst
+      xtchain hdr (DfracOwn 1) nodes dst
     }}}
       #node <-{xtchain_next} v @ E
     {{{
       RET ();
-      xtchain hdr (take (S i) nodes) v ∗
-      xtchain hdr (drop (S i) nodes) dst
+      xtchain hdr (DfracOwn 1) (take (S i) nodes) v ∗
+      xtchain hdr (DfracOwn 1) (drop (S i) nodes) dst
     }}}.
   Proof.
     intros Hlookup.
